examples/QueryStructure/Photoalbum.v
@@ -1,0 +1,122 @@
+Require Import ADTSynthesis.QueryStructure.Automation.AutoDB
+        ADTSynthesis.QueryStructure.Automation.IndexSelection
+        ADTSynthesis.QueryStructure.Specification.SearchTerms.ListInclusion
+        ADTSynthesis.QueryStructure.Specification.SearchTerms.InRange.
+
+(* Collection of Photos. Each photo contains the owner, the list of tags, and
+   the geolocation (latitude and longitude) *)
+
+Definition PHOTOS := "Album".
+Definition USERS := "Users".
+
+Definition USER_ID := "UserId".
+Definition IMAGE_DATA := "ImageData".
+Definition TAGS := "Tags".
+Definition LATITUDE := "Latitude".
+Definition LONGITUDE := "Longitude".
+Definition NAME := "Name".
+
+(* Represents image data by a list of byte characters *)
+Definition DataT := list ascii.
+
+(* Represents a natural number range by a pair of natural numbers *)
+Definition NatRange := prod nat nat.
+
+Definition AlbumSchema :=
+  Query Structure Schema
+    [ relation PHOTOS has
+               schema <USER_ID :: nat,
+                       IMAGE_DATA :: DataT,
+                       TAGS :: list string,
+                       LATITUDE :: nat,
+                       LONGITUDE :: nat>;
+      relation USERS has
+               schema <USER_ID :: nat,
+                       NAME :: string>
+                       where attributes [NAME] depend on [USER_ID]
+    ]
+    enforcing [attribute USER_ID  for PHOTOS references USERS].
+
+Definition AlbumSig : ADTSig :=
+  ADTsignature {
+      Constructor "Init"
+           : unit                             -> rep,
+      Method "AddPhoto"
+           : rep x (AlbumSchema#PHOTOS)       -> rep x bool,
+      Method "AddUser"
+           : rep x (AlbumSchema#USERS)        -> rep x bool,
+      Method "PhotosByLocation"
+           : rep x (NatRange * NatRange)      -> rep x list (AlbumSchema#PHOTOS),
+      Method "PhotosByTags"
+           : rep x list string                -> rep x list (AlbumSchema#PHOTOS),
+      Method "PhotosByUploader"
+           : rep x string                     -> rep x list (AlbumSchema#PHOTOS)
+    }.
+
+Definition AlbumSpec : ADT AlbumSig :=
+  QueryADTRep AlbumSchema {
+    Def Constructor "Init" (_ : unit) : rep := empty,
+
+    update "AddPhoto" (photo : AlbumSchema#PHOTOS) : bool :=
+      Insert photo into PHOTOS,
+
+    update "AddUser" (user : AlbumSchema#USERS) : bool :=
+      Insert user into USERS,
+
+    query "PhotosByLocation" (ranges : NatRange * NatRange) : list (AlbumSchema#PHOTOS) :=
+      (* let (range_latitude, range_longitude) := ranges in *)
+      For (photo in PHOTOS)
+          Where (InRange photo!LATITUDE (fst ranges) /\
+                 InRange photo!LONGITUDE (snd ranges))
+          Return photo,
+          
+    query "PhotosByTags" (search_tags : list string) : list (AlbumSchema#PHOTOS) :=
+      For (photo in PHOTOS)
+          Where (IncludedIn search_tags photo!TAGS)
+          Return photo,
+
+    query "PhotosByUploader" (uploader : string) : list (AlbumSchema#PHOTOS) :=
+      For (user in USERS)
+          (photo in PHOTOS)
+          Where (user!NAME = uploader)
+          Where (photo!USER_ID = user!USER_ID)
+          Return photo
+}.
+
+Definition SharpenedAlbum :
+  Sharpened AlbumSpec.
+Proof.
+  unfold AlbumSpec.
+
+  start honing QueryStructure.
+
+  make simple indexes using [[(RangeIndex, LATITUDE)]; [(EqualityIndex, NAME)]].
+
+  hone constructor "Init".
+  { initializer. }
+
+  hone method "PhotosByLocation".
+  { observer. }
+    
+  hone method "PhotosByTags".
+  { observer. }
+
+  hone method "PhotosByUploader".
+  { observer. }
+
+  hone method "AddPhoto".
+  { insertion. }
+
+  hone method "AddUser".
+  { insertion. }
+
+
+  FullySharpenQueryStructure AlbumSchema Index.
+
+  implement_bag_methods.
+  implement_bag_methods.
+  implement_bag_methods.
+  implement_bag_methods.
+  implement_bag_methods.
+
+Time Defined.
