src/QueryStructure/Automation/SearchTerms/InvertedSearchTerms.v
@@ -16,7 +16,7 @@ Record InvertedSearchTerm
       ItemSearchTerm : @Tuple heading -> bool }.
 
 (* This builds the type of searchterms and the matching function on them *)
-Global Instance IndexedIndexDenotation
+Global Instance InvertedIndexDenotation
        (heading : Heading)
        (index : @Attributes heading)
        (projection : @Tuple heading -> list string)
@@ -32,7 +32,7 @@ Hint Extern 10 (@IndexDenotation InclusionIndex ?heading ?index) =>
 let index_domain := eval hnf in (@Domain heading index) in
 match index_domain with
   | list string =>
-    apply (@IndexedIndexDenotation
+    apply (@InvertedIndexDenotation
              heading index
              (fun tup => GetAttribute tup index ))
 end
