src/QueryStructure/Specification/SearchTerms/InRange.v
@@ -1,0 +1,36 @@
+Require Import Coq.Arith.Compare_dec Omega
+        ADTSynthesis.QueryStructure.Specification.Representation.QueryStructureNotations.
+
+Section RangeClause.  
+  Definition InRange (n : nat) (range : nat * nat) :=
+    (fst range) <= n <= (snd range).
+
+  Definition InRange_dec (n : nat) (range : nat * nat)
+  : {InRange n range} + {~ InRange n range}.
+    refine (
+        if le_dec (fst range) n then
+          if le_dec n (snd range) then
+            left _
+          else
+            right _
+        else
+          right _); unfold InRange in *; intuition eauto.
+  Defined.
+
+  Global Instance DecideableEnsemble_InRange st :
+    DecideableEnsemble (fun a => InRange a st) :=
+    {| dec a := ?[InRange_dec a st] |}.
+  Proof.
+    intros; destruct (InRange_dec a st); intuition eauto; discriminate.
+  Defined.
+
+  Global Instance DecideableEnsemble_InRange_f
+         (A : Type)
+         (f : A -> nat)
+         b :
+    DecideableEnsemble (fun a => InRange (f a) b) :=
+    {| dec a := ?[InRange_dec (f a) b ] |}.
+  Proof.
+    intros; destruct (InRange_dec (f a) b); intuition eauto; discriminate.
+  Defined.
+End RangeClause.
